src/core/DY.Core.Trace.Base.fst
@@ -30,7 +30,6 @@ val empty_trace : #label_t:Type -> trace_ label_t
 let empty_trace = Nil
 
 unfold
-unfold
 val is_empty: #label_t:Type -> trace_ label_t -> bool
 let is_empty = Nil?
 
