src/core/DY.Core.Trace.Manipulation.fst
@@ -571,36 +571,6 @@ let get_state_is_most_recent_state_for prin sess_id tr =
   reveal_opaque (`%get_state) (get_state);
   reveal_opaque (`%is_most_recent_state_for) (is_most_recent_state_for);
   ()
-val is_most_recent_state_for_get_state:
-  prin:principal -> sess_id:state_id ->
-  content_opt:option bytes -> tr:trace ->
-  Lemma
-  (requires is_most_recent_state_for prin sess_id content_opt tr)
-  (ensures (
-    let (content_opt', _) = get_state prin sess_id tr in
-    content_opt == content_opt'
-  ))
-  [SMTPat (is_most_recent_state_for prin sess_id content_opt tr);
-   SMTPat (get_state prin sess_id tr);
-  ]
-let is_most_recent_state_for_get_state prin sess_id content_opt tr =
-  reveal_opaque (`%get_state) (get_state);
-  reveal_opaque (`%is_most_recent_state_for) (is_most_recent_state_for);
-  ()
-
-val get_state_is_most_recent_state_for:
-  prin:principal -> sess_id:state_id ->
-  tr:trace ->
-  Lemma
-  (ensures (
-    let (content_opt, tr_out) = get_state prin sess_id tr in
-    is_most_recent_state_for prin sess_id content_opt tr
-  ))
-  [SMTPat (get_state prin sess_id tr);]
-let get_state_is_most_recent_state_for prin sess_id tr =
-  reveal_opaque (`%get_state) (get_state);
-  reveal_opaque (`%is_most_recent_state_for) (is_most_recent_state_for);
-  ()
 
 #push-options "--ifuel 1"
 val get_state_aux_state_was_set:
